# Real analysis 

***Defintion:*** For arbitrary set A, the outer measure of A, denoted as $m^{*}(A ) = inf\{\sum_{k=0}^\infin \ell(I_k)|A \sub \cup_{k=1}^{\infin}I_k\}$ 

 ***Properties:*** 

1. $m^{*}(\empty) = 0$  

   *Proof:* $\forall \epsilon>0$, $\empty \sub (-\epsilon,\epsilon) \Rightarrow m^{*}(A) ≤ \epsilon$ 

2. $A \sub B \Rightarrow m^{*}(A) ≤ m^{*}(B)$ 

   *Proof:* For arbitray collection of open intervals $\cup_{k=1}^{\infin}I_k$ that contains B, we have $A \sub \cup_{k=1}^{\infin}I_k$. Hence $m^{*}(A)$ must be a lower bound of $\ell(\cup_{k=1}^{\infin}I_k)$ , which imples $m^{*}(A) ≤ m^{*}(B).$

3. $m^{*}(A) = m^{*}(A+y), \forall y \in \R$.

   *Proof:*  For arbitray collection of open intervals $\cup_{k=1}^{\infin}I_k$ that contains A, $\cup_{k=1}^{\infin}I_k+y$ contains $A+y$. Then $m^{*}(A+y) ≤ \ell( \cup_{k=1}^{\infin}I_k+y) = \ell( \cup_{k=1}^{\infin}I_k)$. By the greatest lower bound property, $m^{*}(A+y) ≤ m^{*}(A) $

   Conversely, for arbitray collection of open intervals $\cup_{k=1}^{\infin}I_k$ that contains $A+y$, $\cup_{k=1}^{\infin}I_k-y$ contains $A$. $m^{*}(A) ≤ \ell( \cup_{k=1}^{\infin}I_k-y) = \ell( \cup_{k=1}^{\infin}I_k)$. By the greatest lower bound property, $m^{*}(A)≤ m^{*}(A+y)$.

   In summary, we have $m^{*}(A) = m^{*}(A+y)$

4. $m^{\star}(A) = 0$ if $A$ is countable.

   *Proof:* By countability, label elements in A as $\{a_1,a_2,...,a_n,...\}$. For arbitrary $\epsilon>0$,  construct a collection of open intervals as $I_k = (a_k- \frac{\epsilon}{2^{k+1}},a_k+ \frac{\epsilon}{2^{k+1}})$. Then $a_k \in I_k$ and $A \sub \cup_{k=1}^{\infin}I_k$. $m^*(A) ≤ \sum_{i=1}^\infin\frac{\epsilon}{2^k} = \epsilon$.

5. $m^*(I) = \ell(I)$

   *Proof:* $m^*(I) ≤ \ell(I)$ since $I \sub I$. So it remains to show $m^*(I) ≥ \ell(I)$. Let's start with the closed bounded intervals $[a,b]$

   For arbitrary collection of open intervals $\cup_{k=1}^{\infin}I_k$ that contains I, by compactness, there exists a finite colleciton of open covers that covers $I$.Which is to say, $I \sub \cup_{k=1}^NI_k$. Without loss of generality, let $a \in I_1 := (a_1,b_1)$. If $b_1 > b$, then $b_1-a_1>b-a$ so $\ell(I)$ is a lower bound of $m^*(I),$ and the proof is finished. Otherwise, let $b_1 \sub I_2 := (a_2,b_2) .$ If $b_2 > b, $ then $b_2 - a_2 + b_1 - a_1 > b_2 - a_1 + b_1 - a_2 > b-a$. So $\ell(I)$ is a lower bound of $m^*(I),$ and the proof is finished. This process could continue but will finally end since we only have finite $I_k$, which ends the proof for closed intervals.

   As for open intervals $(a,b),$ given $\epsilon > 0,$ $[a+\epsilon/2,b-\epsilon/2] \sub (a,b) \sub [a-\epsilon/2,b+\epsilon/2]$ where $\epsilon ≤ b-a$. By monotoncity, $m^*([a+\epsilon/2,b-\epsilon/2]) ≤ m^*(a,b) ≤ m^*([a-\epsilon/2,b+\epsilon/2])$   Hence $ b-a - \epsilon≤m^*(I)≤ b-a + \epsilon$ for arbitrary small $\epsilon$. Therefore we will have $m^*(I) = b-a,$ where $I$ is an open interval. 

6. $m^*(\cup_{k=1}^{\infin}A_k) ≤ \sum_{k=1}^{\infin} m^*(A_k)$. This is also called subadditivity. 

   *Proof:* 

   If $m^*(A_k) = \infin$ for some $k$, then the argument is automatically true. 

   It suffices to show $m^*(\cup_{k=1}^{\infin}A_k) ≤ \sum_{k=1}^{\infin}m^*(A_k) + \epsilon$ , for $\epsilon > 0$. For any $A_k$, $\exist \cup_{j=1}^{\infin} I_{k,j}$ contains $A_k$ such that $m^*(A_k) + \epsilon/2^{k} > \sum_{j=1}^{\infin}\ell(I_{k,j})$ . And we also know $\cup_{k=1}^{\infin}A_k \sub \cup_{k=1}^{\infin}\cup_{j=1}^{\infin}I_{j,k} $ Hence, $m^*(\cup_{k=1}^{\infin}A_k) ≤ \sum_{k=1}^\infin \sum_{j=1}^{\infin} \ell(I_{j,k}) ≤ \sum_{k=1}^\infin(m^*(A_k)+ \epsilon/2^{k+1}) = \sum_{k=1}^{\infin}m^*(A) + \epsilon$



***Definition:*** A set E is said to be measurable provided for any set A,
$$
m^*(A ) = m^*(A \cap E) + m^*(A \cap E^C)
$$
***Properties:*** If A and B are two disjoint sets and A is measurable, then $m^*(A \cup B) = m^*(A) + m^*(B)$ 

*Proof:* $m^*(A \cup B) = m^*(A \cup B \cap A) + m^*(A \cup B \cap A^C) = m*(A) + m^*(B)$ 

***Remark:*** By subadditivity, $m^*(A) ≤ m^*(A \cap E) + m^*(A \cap E^C)$ hence to show that a set is measurable, it suffices to show $m^*(A) ≥ m^*(A \cap E) + m^*(A \cap E^C)$ 

***Proposition 1:*** Any set of outer measure 0 is measurable. In particular, any countable set is measurable.

*Proof:* Let $E$ to be the set of outer measure 0. we will have $m^*(A) ≤ m^*(A \cap E) + m^*(A \cap  E^C)$ and $m^*(A \cap E) ≤ m^*(E) = 0$. Hence $ m^*(A ) ≤ m^*(A \cap E^C)$. However by monotonicity, we will also have $m^*(A) ≥ m^*(A \cap E^C)$ Therefore we will have $m^*(A) = m^*(A \cap E^C) = m^*(A\cap E) + m^*(A \cap E^C)$ 

***Proposition 2:*** The union of a finite collection of measurable set is measurable.

***Proof:*** For the $n=2$ case, it suffices to show $m^*(A) ≥ m^*(A \cap (E_1 \cup E_2) )+ m^*(A \cap (E_1 \cup E_2)^C )$

Notice that we have $m^*(A) = m^*(A \cap E_1) + m^*(A \cap E_1^C) = m^*(A \cap E_1) + m^*(A \cap E_1^C \cap E_2 ) + m^*(A \cap E_1^C \cap E_2^C )  $

Since $(A \cap E_1) \cup [A \cap E_1^C \cap E_2] = A \cap [E_1  \cup (E_1^C \cap E_2)] = A \cap [\R  \cap(E_1 \cup E_2)] = A \cap (E_1 \cup E_2)$ 

By subadditivity, we have $m^*(A) ≥ m^*(A \cap (E_1 \cup E_2)) + m^*(A \cap(E_1^C\cap E_2^C)) = m^*(A \cap (E_1 \cup E_2)) + m^*(A \cap (E_1 \cup E_2)^C)$, which is exactly what we wanna show. 

For the general case, we proceed with induction. When $n = 1$, it is trivial. Suppose the conclusion holds for $n = k-1$

When $n = k$ 
$$
\begin{aligned}
m^*(A) &= m^*(A \cap (\cup_{n=1}^{k-1}E_n)) + m^*(A \cap (\cup_{n=1}^{k-1}E_n)^C) \\ &= m^*(A \cap (\cup_{n=1}^{k-1}E_n)) + m^*(A \cap (\cap_{n=1}^{k-1}E_n^C)) \\ &= m^*(A \cap (\cup_{n=1}^{k-1}E_n)) + m^*(A \cap (\cup_{n=1}^{k-1}E_n^C) \cap E_k) + m^*(A \cap (\cap_{n=1}^{k-1}E_n^C) \cap E_k^C)
\\&≥ m^*(A \cap \{(\cup_{n=1}^{k-1}E_n) \cup [(\cup_{n=1}^{k-1}E_n^C) \cap E_k)]\} + m^*(A \cap (\cap_{n=1}^{k-1}E_n^C) \cap E_k^C)
\\&= m^*(A \cap (\cup_{n=1}^{k}E_n)) + m^*(A \cap (\cup_{n=1}^{k}E_n)^C)
\end{aligned}
$$
***Proposition 3:*** Let A be any set and $ \{E_k\}_{k=1}^n$ be a collection of disjoint measurable set. Then $m^*(A \cap(\cup_{k=1} ^nE_k)) = \sum_{k=1}^n m^*(A \cap E_k)$, in particular, $m^*(\cup_{k=1} ^nE_k) = \sum_{k=1}^n m^*(E_k)$,

*Proo:f* For the case of 2, $m^*(A \cap (E_1 \cup E_2)) = m^*[(A \cap (E_1 \cup E_2) ) \cap E_2] +m^*[(A \cap (E_1 \cup E_2) ) \cap E_2^C] = m^*(A \cap E_2) +  m^*[A \cap (E_1 \cap E_2^C) ] = m^*[A \cap E_2 ] + m^*[A \cap E_1 ]  $

In the case of $k = n,$ suppose the conclusion already holds for $n-1,$
$$
\begin{eqnarray}
m^*[A \cap (\cup_{k=1}^n E_n)] &=& m^*\{[A \cap (\cup_{k=1}^n E_k)] \cap E_n \} + m^*\{[A \cap (\cup_{k=1}^n E_k)] \cap E_n^C \} \\&=& m^*(A \cap E_n) + m^*(A \cap (\cup_{k=1}^{n-1}E_k)) \\ &=& m^*(A \cap E_n) + \sum_{k=1}^{n-1} m^*(A \cap E_k) \\&=& \sum_{k=1}^n m^*(A \cap E_k)
\end{eqnarray}
$$
 Replace $A$ by $\R$ we will have the conclusion $m^*(\cup_{k=1} ^nE_k) = \sum_{k=1}^n m^*(E_k)$. 












































































